more

Weidenbach_Book/IsaSAT_Propagate_Conflict.thy
@@ -7,9 +7,6 @@ subsubsection \<open>Refining Propagate And Conflict\<close>
 
 paragraph \<open>Unit Propagation, Inner Loop\<close>
 
-context isasat_input_bounded_nempty
-begin
-
 definition (in -) length_ll_fs :: \<open>nat twl_st_wl \<Rightarrow> nat literal \<Rightarrow> nat\<close> where
   \<open>length_ll_fs = (\<lambda>(_, _, _, _, _, _, W) L. length (W L))\<close>
 
@@ -26,7 +23,7 @@ lemma length_ll_fs_heur_alt_def:
 lemma (in -) get_watched_wl_heur_def: \<open>get_watched_wl_heur = (\<lambda>(M, N, D, Q, W, _). W)\<close>
   by (intro ext, rename_tac x, case_tac x) auto
 
-sepref_thm length_ll_fs_heur_code
+sepref_definition length_ll_fs_heur_code
   is \<open>uncurry (RETURN oo length_ll_fs_heur)\<close>
   :: \<open>[\<lambda>(S, L). nat_of_lit L < length (get_watched_wl_heur S)]\<^sub>a
       isasat_unbounded_assn\<^sup>k *\<^sub>a unat_lit_assn\<^sup>k \<rightarrow> nat_assn\<close>
@@ -35,16 +32,9 @@ sepref_thm length_ll_fs_heur_code
   supply [[goals_limit=1]]
   by sepref
 
-concrete_definition (in -) length_ll_fs_heur_code
-   uses isasat_input_bounded_nempty.length_ll_fs_heur_code.refine_raw
-   is \<open>(uncurry ?f, _) \<in> _\<close>
+declare length_ll_fs_heur_code.refine[sepref_fr_rules]
 
-prepare_code_thms (in -) length_ll_fs_heur_code_def
-
-lemmas length_ll_fs_heur_code_refine[sepref_fr_rules] =
-   length_ll_fs_heur_code.refine[of \<A>\<^sub>i\<^sub>n, OF isasat_input_bounded_nempty_axioms]
-
-sepref_thm length_ll_fs_heur_fast_code
+sepref_definition length_ll_fs_heur_fast_code
   is \<open>uncurry (RETURN oo length_ll_fs_heur)\<close>
   :: \<open>[\<lambda>(S, L). nat_of_lit L < length (get_watched_wl_heur S)]\<^sub>a
       isasat_bounded_assn\<^sup>k *\<^sub>a unat_lit_assn\<^sup>k \<rightarrow>nat_assn\<close>
@@ -53,19 +43,12 @@ sepref_thm length_ll_fs_heur_fast_code
   supply [[goals_limit=1]] length_ll_def[simp]
   by sepref
 
-concrete_definition (in -) length_ll_fs_heur_fast_code
-   uses isasat_input_bounded_nempty.length_ll_fs_heur_fast_code.refine_raw
-   is \<open>(uncurry ?f, _) \<in> _\<close>
-
-prepare_code_thms (in -) length_ll_fs_heur_fast_code_def
-
-lemmas length_ll_fs_heur_fast_code_refine[sepref_fr_rules] =
-   length_ll_fs_heur_fast_code.refine[of \<A>\<^sub>i\<^sub>n, OF isasat_input_bounded_nempty_axioms]
+declare length_ll_fs_heur_fast_code.refine[sepref_fr_rules]
 
 sepref_register unit_propagation_inner_loop_body_wl_heur
 
-sepref_thm unit_propagation_inner_loop_wl_loop_D
-  is \<open>uncurry ((PR_CONST unit_propagation_inner_loop_wl_loop_D_heur))\<close>
+sepref_definition unit_propagation_inner_loop_wl_loop_D
+  is \<open>uncurry unit_propagation_inner_loop_wl_loop_D_heur\<close>
   :: \<open>unat_lit_assn\<^sup>k *\<^sub>a isasat_unbounded_assn\<^sup>d \<rightarrow>\<^sub>a nat_assn *a nat_assn *a isasat_unbounded_assn\<close>
   unfolding unit_propagation_inner_loop_wl_loop_D_heur_def PR_CONST_def
   unfolding watched_by_nth_watched_app watched_app_def[symmetric]
@@ -78,14 +61,7 @@ sepref_thm unit_propagation_inner_loop_wl_loop_D
   supply [[goals_limit=1]]
   by sepref
 
-concrete_definition (in -) unit_propagation_inner_loop_wl_loop_D_code
-   uses isasat_input_bounded_nempty.unit_propagation_inner_loop_wl_loop_D.refine_raw
-   is \<open>(uncurry ?f, _) \<in> _\<close>
-
-prepare_code_thms (in -) unit_propagation_inner_loop_wl_loop_D_code_def
-
-lemmas unit_propagation_inner_loop_wl_loop_D_code_refine[sepref_fr_rules] =
-   unit_propagation_inner_loop_wl_loop_D_code.refine[of \<A>\<^sub>i\<^sub>n, OF isasat_input_bounded_nempty_axioms]
+declare unit_propagation_inner_loop_wl_loop_D.refine[sepref_fr_rules]
 
 lemma unit_propagation_inner_loop_wl_loop_D_heur_fast:
   \<open>length (get_clauses_wl_heur b) \<le> uint64_max \<Longrightarrow>
@@ -94,8 +70,8 @@ lemma unit_propagation_inner_loop_wl_loop_D_heur_fast:
   unfolding unit_propagation_inner_loop_wl_loop_D_heur_inv_def
   by auto
 
-sepref_thm unit_propagation_inner_loop_wl_loop_D_fast
-  is \<open>uncurry ((PR_CONST unit_propagation_inner_loop_wl_loop_D_heur))\<close>
+sepref_definition unit_propagation_inner_loop_wl_loop_D_fast
+  is \<open>uncurry unit_propagation_inner_loop_wl_loop_D_heur\<close>
   :: \<open>[\<lambda>(L, S). length (get_clauses_wl_heur S) \<le> uint64_max]\<^sub>a
       unat_lit_assn\<^sup>k *\<^sub>a isasat_bounded_assn\<^sup>d \<rightarrow> nat_assn *a nat_assn *a isasat_bounded_assn\<close>
   unfolding unit_propagation_inner_loop_wl_loop_D_heur_def PR_CONST_def
@@ -109,16 +85,9 @@ sepref_thm unit_propagation_inner_loop_wl_loop_D_fast
   supply [[goals_limit=1]] unit_propagation_inner_loop_wl_loop_D_heur_fast[intro]
   by sepref
 
-concrete_definition (in -) unit_propagation_inner_loop_wl_loop_D_fast_code
-   uses isasat_input_bounded_nempty.unit_propagation_inner_loop_wl_loop_D_fast.refine_raw
-   is \<open>(uncurry ?f, _) \<in> _\<close>
+declare unit_propagation_inner_loop_wl_loop_D_fast.refine[sepref_fr_rules]
 
-prepare_code_thms (in -) unit_propagation_inner_loop_wl_loop_D_fast_code_def
-
-lemmas unit_propagation_inner_loop_wl_loop_D_fast_code_refine[sepref_fr_rules] =
-   unit_propagation_inner_loop_wl_loop_D_fast_code.refine[of \<A>\<^sub>i\<^sub>n, OF isasat_input_bounded_nempty_axioms]
-
-lemma (in isasat_input_ops) unit_propagation_inner_loop_wl_loop_D_heur_alt_def:
+lemma unit_propagation_inner_loop_wl_loop_D_heur_alt_def:
   \<open>unit_propagation_inner_loop_wl_loop_D_heur L S\<^sub>0 = do {
     ASSERT (nat_of_lit L < length (get_watched_wl_heur S\<^sub>0));
     let n = length (watched_by_int S\<^sub>0 L);
@@ -136,7 +105,7 @@ lemma (in isasat_input_ops) unit_propagation_inner_loop_wl_loop_D_heur_alt_def:
 sepref_register length_ll_fs_heur
 
 sepref_register unit_propagation_inner_loop_wl_loop_D_heur
-sepref_thm cut_watch_list_heur2
+sepref_definition cut_watch_list_heur2_code
   is \<open>uncurry3 cut_watch_list_heur2\<close>
   :: \<open>nat_assn\<^sup>k *\<^sub>a nat_assn\<^sup>k *\<^sub>a unat_lit_assn\<^sup>k *\<^sub>a
      isasat_unbounded_assn\<^sup>d \<rightarrow>\<^sub>a isasat_unbounded_assn\<close>
@@ -145,16 +114,9 @@ sepref_thm cut_watch_list_heur2
   update_ll_def[symmetric] nth_rll_def[symmetric] shorten_take_ll_def[symmetric]
   by sepref
 
-concrete_definition (in -) cut_watch_list_heur2_code
-   uses isasat_input_bounded_nempty.cut_watch_list_heur2.refine_raw
-   is \<open>(uncurry3 ?f, _)\<in>_\<close>
+declare cut_watch_list_heur2_code.refine[sepref_fr_rules]
 
-prepare_code_thms (in -) cut_watch_list_heur2_code_def
-
-lemmas cut_watch_list_heur2_refine[sepref_fr_rules] =
-   cut_watch_list_heur2_code.refine[of \<A>\<^sub>i\<^sub>n, OF isasat_input_bounded_nempty_axioms]
-
-sepref_thm cut_watch_list_heur2_fast
+sepref_definition cut_watch_list_heur2_fast_code
   is \<open>uncurry3 cut_watch_list_heur2\<close>
   :: \<open>nat_assn\<^sup>k *\<^sub>a nat_assn\<^sup>k *\<^sub>a unat_lit_assn\<^sup>k *\<^sub>a
      isasat_bounded_assn\<^sup>d \<rightarrow>\<^sub>a isasat_bounded_assn\<close>
@@ -163,48 +125,26 @@ sepref_thm cut_watch_list_heur2_fast
   update_ll_def[symmetric] nth_rll_def[symmetric] shorten_take_ll_def[symmetric]
   by sepref
 
-concrete_definition (in -) cut_watch_list_heur2_fast_code
-   uses isasat_input_bounded_nempty.cut_watch_list_heur2_fast.refine_raw
-   is \<open>(uncurry3 ?f, _)\<in>_\<close>
+declare cut_watch_list_heur2_fast_code.refine[sepref_fr_rules]
 
-prepare_code_thms (in -) cut_watch_list_heur2_fast_code_def
-
-lemmas cut_watch_list_heur2_fast_refine[sepref_fr_rules] =
-   cut_watch_list_heur2_fast_code.refine[of \<A>\<^sub>i\<^sub>n, OF isasat_input_bounded_nempty_axioms]
-
-
-sepref_thm unit_propagation_inner_loop_wl_D
-  is \<open>uncurry (PR_CONST unit_propagation_inner_loop_wl_D_heur)\<close>
+sepref_definition unit_propagation_inner_loop_wl_D
+  is \<open>uncurry unit_propagation_inner_loop_wl_D_heur\<close>
   :: \<open>unat_lit_assn\<^sup>k *\<^sub>a isasat_unbounded_assn\<^sup>d \<rightarrow>\<^sub>a isasat_unbounded_assn\<close>
   supply [[goals_limit=1]]
   unfolding PR_CONST_def unit_propagation_inner_loop_wl_D_heur_def
   by sepref
 
-concrete_definition (in -) unit_propagation_inner_loop_wl_D_code
-   uses isasat_input_bounded_nempty.unit_propagation_inner_loop_wl_D.refine_raw
-   is \<open>(uncurry ?f, _)\<in>_\<close>
+declare unit_propagation_inner_loop_wl_D.refine[sepref_fr_rules]
 
-prepare_code_thms (in -) unit_propagation_inner_loop_wl_D_code_def
-
-lemmas unit_propagation_inner_loop_wl_D_code_refine[sepref_fr_rules] =
-   unit_propagation_inner_loop_wl_D_code.refine[of \<A>\<^sub>i\<^sub>n, OF isasat_input_bounded_nempty_axioms]
-
-sepref_thm unit_propagation_inner_loop_wl_D_fast
-  is \<open>uncurry (PR_CONST unit_propagation_inner_loop_wl_D_heur)\<close>
+sepref_definition unit_propagation_inner_loop_wl_D_fast
+  is \<open>uncurry unit_propagation_inner_loop_wl_D_heur\<close>
   :: \<open>[\<lambda>(L, S). length (get_clauses_wl_heur S) \<le> uint64_max]\<^sub>a
         unat_lit_assn\<^sup>k *\<^sub>a isasat_bounded_assn\<^sup>d \<rightarrow> isasat_bounded_assn\<close>
   supply [[goals_limit=1]]
   unfolding PR_CONST_def unit_propagation_inner_loop_wl_D_heur_def
   by sepref
 
-concrete_definition (in -) unit_propagation_inner_loop_wl_D_fast_code
-   uses isasat_input_bounded_nempty.unit_propagation_inner_loop_wl_D_fast.refine_raw
-   is \<open>(uncurry ?f, _)\<in>_\<close>
-
-prepare_code_thms (in -) unit_propagation_inner_loop_wl_D_fast_code_def
-
-lemmas unit_propagation_inner_loop_wl_D_fast_code_refine[sepref_fr_rules] =
-   unit_propagation_inner_loop_wl_D_fast_code.refine[of \<A>\<^sub>i\<^sub>n, OF isasat_input_bounded_nempty_axioms]
+declare unit_propagation_inner_loop_wl_D_fast.refine[sepref_fr_rules]
 
 
 paragraph \<open>Unit propagation, Outer Loop\<close>
@@ -213,11 +153,11 @@ lemma select_and_remove_from_literals_to_update_wl_heur_alt_def:
   \<open>select_and_remove_from_literals_to_update_wl_heur =
    (\<lambda>(M', N', D', j, W', vm, \<phi>, clvls, cach, lbd, outl, stats, fast_ema, slow_ema, ccount,
        vdom, lcount). do {
-      ASSERT(j < length M');
+      ASSERT(j < length (fst M'));
       ASSERT(j + 1 \<le> uint32_max);
-      let L = - rev_trail_nth M' j;
+      L \<leftarrow> isa_trail_nth M' j;
       RETURN ((M', N', D', j+1, W', vm, \<phi>, clvls, cach, lbd, outl, stats, fast_ema, slow_ema, ccount,
-       vdom, lcount), L)
+       vdom, lcount), -L)
      })
     \<close>
   unfolding select_and_remove_from_literals_to_update_wl_heur_def
@@ -225,7 +165,7 @@ lemma select_and_remove_from_literals_to_update_wl_heur_alt_def:
   apply (rename_tac S; case_tac S)
   by (auto intro!: ext simp: rev_trail_nth_def Let_def)
 
-sepref_thm select_and_remove_from_literals_to_update_wl_code
+sepref_definition select_and_remove_from_literals_to_update_wl_code
   is \<open>select_and_remove_from_literals_to_update_wl_heur\<close>
   :: \<open>isasat_unbounded_assn\<^sup>d \<rightarrow>\<^sub>a isasat_unbounded_assn *a unat_lit_assn\<close>
   supply [[goals_limit=1]] uint32_nat_assn_plus[sepref_fr_rules]
@@ -234,18 +174,9 @@ sepref_thm select_and_remove_from_literals_to_update_wl_code
   supply [[goals_limit = 1]]
   by sepref
 
-concrete_definition (in -) select_and_remove_from_literals_to_update_wl_code
-   uses isasat_input_bounded_nempty.select_and_remove_from_literals_to_update_wl_code.refine_raw
-   is \<open>(?f, _)\<in>_\<close>
+declare select_and_remove_from_literals_to_update_wl_code.refine[sepref_fr_rules]
 
-prepare_code_thms (in -) select_and_remove_from_literals_to_update_wl_code_def
-
-lemmas select_and_remove_from_literals_to_update_wl_code_refine[sepref_fr_rules] =
-   select_and_remove_from_literals_to_update_wl_code.refine[of \<A>\<^sub>i\<^sub>n,
-     OF isasat_input_bounded_nempty_axioms]
-
-
-sepref_thm select_and_remove_from_literals_to_update_wlfast_code
+sepref_definition select_and_remove_from_literals_to_update_wlfast_code
   is \<open>select_and_remove_from_literals_to_update_wl_heur\<close>
   :: \<open>isasat_bounded_assn\<^sup>d \<rightarrow>\<^sub>a isasat_bounded_assn *a unat_lit_assn\<close>
   supply [[goals_limit=1]] uint32_nat_assn_plus[sepref_fr_rules]
@@ -254,81 +185,57 @@ sepref_thm select_and_remove_from_literals_to_update_wlfast_code
   supply [[goals_limit = 1]]
   by sepref
 
-concrete_definition (in -) select_and_remove_from_literals_to_update_wlfast_code
-   uses isasat_input_bounded_nempty.select_and_remove_from_literals_to_update_wlfast_code.refine_raw
-   is \<open>(?f, _)\<in>_\<close>
+declare select_and_remove_from_literals_to_update_wlfast_code.refine[sepref_fr_rules]
 
-prepare_code_thms (in -) select_and_remove_from_literals_to_update_wlfast_code_def
-
-lemmas select_and_remove_from_literals_to_update_wlfast_code_refine[sepref_fr_rules] =
-   select_and_remove_from_literals_to_update_wlfast_code.refine[of \<A>\<^sub>i\<^sub>n,
-     OF isasat_input_bounded_nempty_axioms]
-
-definition (in -) literals_to_update_wl_literals_to_update_wl_empty :: \<open>twl_st_wl_heur \<Rightarrow> bool\<close> where
+definition  literals_to_update_wl_literals_to_update_wl_empty :: \<open>twl_st_wl_heur \<Rightarrow> bool\<close> where
   \<open>literals_to_update_wl_literals_to_update_wl_empty S \<longleftrightarrow>
-    literals_to_update_wl_heur S < length (get_trail_wl_heur S)\<close>
+    literals_to_update_wl_heur S < isa_length_trail (get_trail_wl_heur S)\<close>
 
 
 lemma literals_to_update_wl_literals_to_update_wl_empty_alt_def:
   \<open>literals_to_update_wl_literals_to_update_wl_empty =
     (\<lambda>(M', N', D', j, W', vm, \<phi>, clvls, cach, lbd, outl, stats, fast_ema, slow_ema, ccount,
-       vdom, lcount). j < length_u M')\<close>
-  unfolding literals_to_update_wl_literals_to_update_wl_empty_def
-  by (auto intro!: ext)
+       vdom, lcount). j < isa_length_trail M')\<close>
+  unfolding literals_to_update_wl_literals_to_update_wl_empty_def isa_length_trail_def
+  by (auto intro!: ext split: prod.splits)
 
-sepref_thm literals_to_update_wl_literals_to_update_wl_empty_code
+sepref_definition literals_to_update_wl_literals_to_update_wl_empty_code
   is \<open>RETURN o literals_to_update_wl_literals_to_update_wl_empty\<close>
-  :: \<open>isasat_unbounded_assn\<^sup>k \<rightarrow>\<^sub>a bool_assn\<close>
+  :: \<open>[\<lambda>S. isa_length_trail_pre (get_trail_wl_heur S)]\<^sub>a isasat_unbounded_assn\<^sup>k \<rightarrow> bool_assn\<close>
   unfolding literals_to_update_wl_literals_to_update_wl_empty_alt_def
     isasat_unbounded_assn_def
   by sepref
 
-concrete_definition (in -) literals_to_update_wl_literals_to_update_wl_empty_code
-   uses isasat_input_bounded_nempty.literals_to_update_wl_literals_to_update_wl_empty_code.refine_raw
-   is \<open>(?f,_)\<in>_\<close>
+declare literals_to_update_wl_literals_to_update_wl_empty_code.refine[sepref_fr_rules]
 
-prepare_code_thms (in -) literals_to_update_wl_literals_to_update_wl_empty_code_def
-
-lemmas literals_to_update_wl_literals_to_update_wl_empty_code_hnr[sepref_fr_rules] =
-   literals_to_update_wl_literals_to_update_wl_empty_code.refine[of \<A>\<^sub>i\<^sub>n, OF isasat_input_bounded_nempty_axioms]
-
-sepref_thm literals_to_update_wl_literals_to_update_wl_empty_fast_code
+sepref_definition literals_to_update_wl_literals_to_update_wl_empty_fast_code
   is \<open>RETURN o literals_to_update_wl_literals_to_update_wl_empty\<close>
-  :: \<open>isasat_bounded_assn\<^sup>k \<rightarrow>\<^sub>a bool_assn\<close>
+  :: \<open>[\<lambda>S. isa_length_trail_pre (get_trail_wl_heur S)]\<^sub>a isasat_bounded_assn\<^sup>k \<rightarrow> bool_assn\<close>
   unfolding literals_to_update_wl_literals_to_update_wl_empty_alt_def
     isasat_bounded_assn_def
   by sepref
 
-concrete_definition (in -) literals_to_update_wl_literals_to_update_wl_empty_fast_code
-   uses isasat_input_bounded_nempty.literals_to_update_wl_literals_to_update_wl_empty_fast_code.refine_raw
-   is \<open>(?f,_)\<in>_\<close>
-
-prepare_code_thms (in -) literals_to_update_wl_literals_to_update_wl_empty_fast_code_def
-
-lemmas literals_to_update_wl_literals_to_update_wl_empty_fast_code_hnr[sepref_fr_rules] =
-   literals_to_update_wl_literals_to_update_wl_empty_fast_code.refine[of \<A>\<^sub>i\<^sub>n, OF isasat_input_bounded_nempty_axioms]
+declare literals_to_update_wl_literals_to_update_wl_empty_fast_code.refine[sepref_fr_rules]
 
 sepref_register literals_to_update_wl_literals_to_update_wl_empty
   select_and_remove_from_literals_to_update_wl_heur
-  unit_propagation_inner_loop_wl_D_heur
 
-sepref_thm unit_propagation_outer_loop_wl_D
-  is \<open>PR_CONST unit_propagation_outer_loop_wl_D_heur\<close>
+lemma unit_propagation_outer_loop_wl_D_invI:
+  \<open>unit_propagation_outer_loop_wl_D_heur_inv S\<^sub>0 S \<Longrightarrow>
+    isa_length_trail_pre (get_trail_wl_heur S)\<close>
+  unfolding unit_propagation_outer_loop_wl_D_heur_inv_def
+  by blast
+
+sepref_definition unit_propagation_outer_loop_wl_D
+  is \<open>unit_propagation_outer_loop_wl_D_heur\<close>
   :: \<open>isasat_unbounded_assn\<^sup>d \<rightarrow>\<^sub>a isasat_unbounded_assn\<close>
   supply [[goals_limit=1]]
-  apply (subst PR_CONST_def)
+    unit_propagation_outer_loop_wl_D_invI[intro]
   unfolding unit_propagation_outer_loop_wl_D_heur_def
     literals_to_update_wl_literals_to_update_wl_empty_def[symmetric]
   by sepref
 
-concrete_definition (in -) unit_propagation_outer_loop_wl_D
-   uses isasat_input_bounded_nempty.unit_propagation_outer_loop_wl_D.refine_raw
-   is \<open>(?f,_)\<in>_\<close>
-
-prepare_code_thms (in -) unit_propagation_outer_loop_wl_D_def
-
-lemmas unit_propagation_outer_loop_wl_D[sepref_fr_rules] =
-   unit_propagation_outer_loop_wl_D.refine[of \<A>\<^sub>i\<^sub>n, OF isasat_input_bounded_nempty_axioms]
+declare unit_propagation_outer_loop_wl_D.refine[sepref_fr_rules]
 
 lemma unit_propagation_outer_loop_wl_D_heur_fast:
   \<open>length (get_clauses_wl_heur x) \<le> uint64_max \<Longrightarrow>
@@ -339,24 +246,15 @@ lemma unit_propagation_outer_loop_wl_D_heur_fast:
        length (get_clauses_wl_heur s') \<le> uint64_max\<close>
   by (auto simp: unit_propagation_outer_loop_wl_D_heur_inv_def)
 
-sepref_thm unit_propagation_outer_loop_wl_D_fast
-  is \<open>PR_CONST unit_propagation_outer_loop_wl_D_heur\<close>
+sepref_definition unit_propagation_outer_loop_wl_D_fast
+  is \<open>unit_propagation_outer_loop_wl_D_heur\<close>
   :: \<open>[\<lambda>S. length (get_clauses_wl_heur S) \<le> uint64_max]\<^sub>a isasat_bounded_assn\<^sup>d \<rightarrow> isasat_bounded_assn\<close>
   supply [[goals_limit=1]] unit_propagation_outer_loop_wl_D_heur_fast[intro]
-  apply (subst PR_CONST_def)
+    unit_propagation_outer_loop_wl_D_invI[intro]
   unfolding unit_propagation_outer_loop_wl_D_heur_def
     literals_to_update_wl_literals_to_update_wl_empty_def[symmetric]
   by sepref
 
-concrete_definition (in -) unit_propagation_outer_loop_wl_D_fast
-   uses isasat_input_bounded_nempty.unit_propagation_outer_loop_wl_D_fast.refine_raw
-   is \<open>(?f,_)\<in>_\<close>
-
-prepare_code_thms (in -) unit_propagation_outer_loop_wl_D_fast_def
-
-lemmas unit_propagation_outer_loop_wl_D_fast[sepref_fr_rules] =
-   unit_propagation_outer_loop_wl_D_fast.refine[of \<A>\<^sub>i\<^sub>n, OF isasat_input_bounded_nempty_axioms]
-
-end
+declare unit_propagation_outer_loop_wl_D_fast.refine[sepref_fr_rules]
 
 end
